proof/garble/equivFake.ec
@@ -34,6 +34,7 @@ module Fake(A:Garble.Adv) = {
   var t : bool array
   var v : bool array
   var xx : tokens
+  var randG : (int*bool*bool, token) map
   var a : int
   var b : int
   var i : int
@@ -45,14 +46,14 @@ module Fake(A:Garble.Adv) = {
   var kpub : (int*bool, token) map
 (*End DKC Var*)
 
-  fun query(rand:bool, alpha:bool, bet:bool) : token = {
+  fun query(rand:bool, alpha:bool, bet:bool) : unit = {
     var ttt : token;
     var pos : bool;
     var input : int*bool;
     var output : int*bool;
     var ra : bool;
     var ki : token;
-    var ko : token;
+    var tok : token;
     var zz : token;
 
     ttt = tweak g (t.[a]^^alpha) (t.[b]^^bet);
@@ -66,12 +67,9 @@ module Fake(A:Garble.Adv) = {
 
 
     (*DKC encrypt*)
-        if (! (in_dom input kpub)) kpub.[input] = $DKC.genRandKeyLast (snd input);
-        if (! (in_dom output kpub)) kpub.[output] = $DKC.genRandKeyLast (snd output);
-        if (! (in_dom output r)) r.[output] = $DKC.genRandKey;
+        tok = $DKC.genRandKey;
         ki = proj kpub.[input];
-        ko = proj kpub.[output];
-        zz = DKC.encode ttt (proj kpub.[input]) ksec (proj r.[output]);
+        zz = DKC.encode ttt (proj kpub.[input]) ksec tok;
     (*End DKC encrypt*)
      
 
@@ -83,7 +81,6 @@ module Fake(A:Garble.Adv) = {
     ans = sub ans 0 ((length ans) - 1);
     pp.[g] = setGateVal pp.[g] ((t.[a]^^alpha), (t.[b]^^bet)) zz;
     xx = setTok xx g (v.[a]^^alpha) ki;
-    return ko;
   }
 
   fun garb(yy:token, alpha:bool, bet:bool) : unit = {
@@ -96,9 +93,14 @@ module Fake(A:Garble.Adv) = {
 
   fun garbD(alpha:bool, bet:bool) : token = {
     var yy : token;
-    yy = $DKC.genRandKey;
+    yy = proj randG.[(g,alpha,bet)];
     garb(yy, alpha, bet);
     return yy;
+  }
+
+  fun preGarbD(alpha:bool, bet:bool) : unit = {
+    var yy : token;
+    randG.[(g,alpha,bet)] = $DKC.genRandKey;
   }
 
   fun garble() : unit = {
@@ -125,20 +127,25 @@ module Fake(A:Garble.Adv) = {
       a = aa.[g];
       b = bb.[g];
       if (b = borne - 1) {
-        tok = query(false, false, true);
-        tok = query(true, true, true);
+        query(false, false, true);
+        query(true, true, true);
+        preGarbD(true, false);
+      } else {
+        preGarbD(true, false);
+        preGarbD(false, true);
+        preGarbD(true, true);
       }
       g = g + 1;
     }
 
     i = 0;
     while (i < n+q) {
+      tok = $DKC.genRandKeyLast (! t.[i]);
       if (getTok xx i true = void /\ i <> 0) {
-        tok = $DKC.genRandKeyLast (! t.[i]);
         xx = setTok xx i true tok;
       }
+      tok = $DKC.genRandKeyLast (t.[i]);
       if (getTok xx i false = void) {
-        tok = $DKC.genRandKeyLast (t.[i]);
         xx = setTok xx i false tok;
       }
       i = i + 1;
@@ -150,9 +157,9 @@ module Fake(A:Garble.Adv) = {
       b = bb.[g];
       garb(getTok xx g v.[g], false, false);
       if (b <> borne - 1) {
-        tok = garbD(true, false);
         tok = garbD(false, true);
         tok = garbD(true, true);
+        tok = garbD(true, false);
       } else {
         tok = garbD(true, false);
       }
@@ -204,7 +211,7 @@ lemma fakeEq :
       : (glob ADV){1} = (glob ADV){2} /\
       (!DKC.Dkc.b{1}) /\ (AdvAda.l{1}=borne-1) ==> res{1} = res{2}
     ].
-proof.
+proof strict.
   intros ADV.
   fun.
   inline {1} GameAda(DKC.Dkc, ADV).A.work.
@@ -213,6 +220,7 @@ proof.
   inline {1} AdvAda(ADV, DKC.Dkc).query.
   inline {1} AdvAda(ADV, DKC.Dkc).garbD.
   inline {1} AdvAda(ADV, DKC.Dkc).garb.
+  inline {1} AdvAda(ADV, DKC.Dkc).preGarbD.
   inline {1} DKC.Dkc.preInit.
   inline {1} DKC.Dkc.get_challenge.
   inline {1} DKC.Dkc.initialize.
@@ -222,6 +230,7 @@ proof.
   inline {2} Fake(ADV).query.
   inline {2} Fake(ADV).garbD.
   inline {2} Fake(ADV).garb.
+  inline {2} Fake(ADV).preGarbD.
 
   swap{1} 8 -7.
 
@@ -243,33 +252,38 @@ proof.
   wp.
 
   while (
-    (glob ADV){1} = (glob ADV){2} /\
-    length AdvAda.xx{1} = AdvAda.n{1}+AdvAda.q{1} /\
-    length AdvAda.t{1} = AdvAda.n{1}+AdvAda.q{1} /\
-    AdvAda.xx{1} = Fake.xx{2} /\
-    AdvAda.t{1} = Fake.t{2}/\
-    AdvAda.v{1} = Fake.v{2}/\
-    AdvAda.n{1} = Fake.n{2}/\
-    AdvAda.m{1} = Fake.m{2}/\
-    AdvAda.q{1} = Fake.q{2}/\
-    AdvAda.aa{1} = Fake.aa{2}/\
-    AdvAda.bb{1} = Fake.bb{2}/\
-    AdvAda.fc{1} = Fake.f1{2}/\
-    (AdvAda.c{1} = DKC.Dkc.b{1}) = PrvInd.b{2}/\
-    AdvAda.xc{1} = Fake.x1{2}/\
-    (*Fake.f1{2} = (Fake.n{2}, Fake.m{2}, Fake.q{2}, Fake.aa{2}, Fake.bb{2}, Fake.gg{2}) /\*)
-    borne = Fake.n{2} + Fake.q{2} /\
-    AdvAda.l{1} = borne-1 /\
+      (glob ADV){1} = (glob ADV){2} /\
+      length AdvAda.xx{1} = AdvAda.n{1}+AdvAda.q{1} /\
+      length AdvAda.t{1} = AdvAda.n{1}+AdvAda.q{1} /\
+      AdvAda.xx{1} = Fake.xx{2} /\
+      AdvAda.t{1} = Fake.t{2}/\
+      AdvAda.v{1} = Fake.v{2}/\
+      AdvAda.n{1} = Fake.n{2}/\
+      AdvAda.m{1} = Fake.m{2}/\
+      AdvAda.q{1} = Fake.q{2}/\
+      AdvAda.aa{1} = Fake.aa{2}/\
+      AdvAda.bb{1} = Fake.bb{2}/\
+      AdvAda.randG{1} = Fake.randG{2}/\
+      AdvAda.pp{1} = Fake.pp{2}/\
+      AdvAda.fc{1} = Fake.f1{2}/\
+      (AdvAda.c{1} = DKC.Dkc.b{1}) = PrvInd.b{2}/\
+      AdvAda.xc{1} = Fake.x1{2}/\
+      Fake.n{2} > 1/\
+      Fake.m{2} > 0/\
+      Fake.q{2} > 0/\
+      (*Fake.f1{2} = (Fake.n{2}, Fake.m{2}, Fake.q{2}, Fake.aa{2}, Fake.bb{2}, Fake.gg{2}) /\*)
+      borne = Fake.n{2} + Fake.q{2} /\
+      AdvAda.l{1} = borne-1 /\
     (forall i, i >= Fake.n{2} => i < Fake.n{2}+Fake.q{2} => Fake.aa{2}.[i] >= 0 /\
            Fake.bb{2}.[i] < borne /\ Fake.bb{2}.[i] < i /\ Fake.aa{2}.[i] < Fake.bb{2}.[i]) /\
+    (forall g, if (AdvAda.bb{1}.[g] = borne-1 /\ evalGate AdvAda.gg{1}.[g]
+      ((!AdvAda.v{1}.[AdvAda.aa{1}.[g]]), false) = evalGate AdvAda.gg{1}.[g] ((!AdvAda.v{1}.[AdvAda.aa{1}.[g]]), true)) then
+        AdvAda.yy{1}.[g]=proj Fake.randG{2}.[(g, true, false)] else true)/\
 
     AdvAda.g{1} = Fake.g{2} /\
       Fake.g{2} > Fake.n{2} /\
-    AdvAda.pp{1} = Fake.pp{2} /\
     true
   ).
-    wp.
-    
     seq 6 6 : (
       (glob ADV){1} = (glob ADV){2} /\
       length AdvAda.xx{1} = AdvAda.n{1}+AdvAda.q{1} /\
@@ -282,16 +296,27 @@ proof.
       AdvAda.q{1} = Fake.q{2}/\
       AdvAda.aa{1} = Fake.aa{2}/\
       AdvAda.bb{1} = Fake.bb{2}/\
+      AdvAda.randG{1} = Fake.randG{2}/\
+      AdvAda.pp{1} = Fake.pp{2}/\
       AdvAda.fc{1} = Fake.f1{2}/\
       (AdvAda.c{1} = DKC.Dkc.b{1}) = PrvInd.b{2}/\
       AdvAda.xc{1} = Fake.x1{2}/\
+      Fake.n{2} > 1/\
+      Fake.m{2} > 0/\
+      Fake.q{2} > 0/\
       (*Fake.f1{2} = (Fake.n{2}, Fake.m{2}, Fake.q{2}, Fake.aa{2}, Fake.bb{2}, Fake.gg{2}) /\*)
       borne = Fake.n{2} + Fake.q{2} /\
       AdvAda.l{1} = borne-1 /\
     (forall i, i >= Fake.n{2} => i < Fake.n{2}+Fake.q{2} => Fake.aa{2}.[i] >= 0 /\
            Fake.bb{2}.[i] < borne /\ Fake.bb{2}.[i] < i /\ Fake.aa{2}.[i] < Fake.bb{2}.[i]) /\
+    (forall g, if (AdvAda.bb{1}.[g] = borne-1 /\ evalGate AdvAda.gg{1}.[g]
+      ((!AdvAda.v{1}.[AdvAda.aa{1}.[g]]), false) = evalGate AdvAda.gg{1}.[g] ((!AdvAda.v{1}.[AdvAda.aa{1}.[g]]), true)) then
+        AdvAda.yy{1}.[g]=proj Fake.randG{2}.[(g, true, false)] else true)/\
 
 
+    (if (AdvAda.b{1} = borne-1 /\ evalGate AdvAda.gg{1}.[Fake.g{2}]
+      ((!AdvAda.v{1}.[AdvAda.a{1}]), false) = evalGate AdvAda.gg{1}.[Fake.g{2}] ((!AdvAda.v{1}.[AdvAda.a{1}]), true)) then
+        AdvAda.yy{1}.[Fake.g{2}]=proj Fake.randG{2}.[(Fake.g{2}, true, false)] else true)/\
       AdvAda.g{1} = Fake.g{2} /\
       Fake.g{2} > Fake.n{2} /\
       AdvAda.a{1} = Fake.a{2} /\
@@ -303,20 +328,171 @@ proof.
     if;first smt.
       (*IF TRUE*)
       rcondt{1} 4;first (intros _;wp;skip;smt).
-      rcondt{1} 13;first (intros _;wp;rnd;wp;skip;smt).
-      rcondt{1} 22;first (intros _;wp;rnd;wp;rnd;wp;skip;smt).
-      wp;rnd;wp;rnd;wp;rnd;wp;skip;progress assumption;[smt| |smt| ].
-      congr. (*BUG*)
+      rcondt{1} 13;first (intros _;wp;skip;smt).
+      rcondf{1} 19;first (intros _;wp;skip;smt).
+      rcondt{1} 22;first (intros _;wp;skip;smt).
+      wp;skip;progress assumption;smt.
       (*IF FALSE*)
       rcondf{1} 1;first (intros _;skip;smt).
-      rcondt{1} 4;first (intros _;wp;skip;smt).
-      wp;rnd;wp;skip;progress assumption;smt.
+      cfold{1} 1?1.
+      (wp;skip;progress assumption;first rewrite H7);smt.
+  
+
+  wp.
+
+
+
+  while (
+      (glob ADV){1} = (glob ADV){2} /\
+      length AdvAda.xx{1} = AdvAda.n{1}+AdvAda.q{1} /\
+      length AdvAda.t{1} = AdvAda.n{1}+AdvAda.q{1} /\
+      AdvAda.xx{1} = Fake.xx{2} /\
+      AdvAda.t{1} = Fake.t{2}/\
+      AdvAda.v{1} = Fake.v{2}/\
+      AdvAda.n{1} = Fake.n{2}/\
+      AdvAda.m{1} = Fake.m{2}/\
+      AdvAda.q{1} = Fake.q{2}/\
+      AdvAda.aa{1} = Fake.aa{2}/\
+      AdvAda.bb{1} = Fake.bb{2}/\
+      AdvAda.randG{1} = Fake.randG{2}/\
+      AdvAda.pp{1} = Fake.pp{2}/\
+      AdvAda.fc{1} = Fake.f1{2}/\
+      (AdvAda.c{1} = DKC.Dkc.b{1}) = PrvInd.b{2}/\
+      AdvAda.xc{1} = Fake.x1{2}/\
+      Fake.n{2} > 1/\
+      Fake.m{2} > 0/\
+      Fake.q{2} > 0/\
+      (*Fake.f1{2} = (Fake.n{2}, Fake.m{2}, Fake.q{2}, Fake.aa{2}, Fake.bb{2}, Fake.gg{2}) /\*)
+      borne = Fake.n{2} + Fake.q{2} /\
+      AdvAda.l{1} = borne-1 /\
+    (forall i, i >= Fake.n{2} => i < Fake.n{2}+Fake.q{2} => Fake.aa{2}.[i] >= 0 /\
+           Fake.bb{2}.[i] < borne /\ Fake.bb{2}.[i] < i /\ Fake.aa{2}.[i] < Fake.bb{2}.[i]) /\
+    (forall g, if (AdvAda.bb{1}.[g] = borne-1 /\ evalGate AdvAda.gg{1}.[g]
+      ((!AdvAda.v{1}.[AdvAda.aa{1}.[g]]), false) = evalGate AdvAda.gg{1}.[g] ((!AdvAda.v{1}.[AdvAda.aa{1}.[g]]), true)) then
+        AdvAda.yy{1}.[g]=proj Fake.randG{2}.[(g, true, false)] else true)/\
+
+    AdvAda.i{1} = Fake.i{2} /\
+      0 <= Fake.i{2} /\
+    true
+  ).
+  wp.
+  rnd.
+  wp.
+  rnd.
+  skip.
+  progress assumption;last 4 smt.
+    delta setTok;simplify;rewrite ! set_length;try assumption;smt.
+    smt.
+    delta setTok;simplify;rewrite ! set_length;try assumption;smt.
+  wp.
+
+  while (
+      (glob ADV){1} = (glob ADV){2} /\
+      length AdvAda.xx{1} = AdvAda.n{1}+AdvAda.q{1} /\
+      length AdvAda.t{1} = AdvAda.n{1}+AdvAda.q{1} /\
+      AdvAda.xx{1} = Fake.xx{2} /\
+      AdvAda.t{1} = Fake.t{2}/\
+      AdvAda.v{1} = Fake.v{2}/\
+      AdvAda.n{1} = Fake.n{2}/\
+      AdvAda.m{1} = Fake.m{2}/\
+      AdvAda.q{1} = Fake.q{2}/\
+      AdvAda.aa{1} = Fake.aa{2}/\
+      AdvAda.bb{1} = Fake.bb{2}/\
+      AdvAda.randG{1} = Fake.randG{2}/\
+      AdvAda.pp{1} = Fake.pp{2}/\
+      AdvAda.fc{1} = Fake.f1{2}/\
+      (AdvAda.c{1} = DKC.Dkc.b{1}) = PrvInd.b{2}/\
+      AdvAda.xc{1} = Fake.x1{2}/\
+      Fake.n{2} > 1/\
+      Fake.m{2} > 0/\
+      Fake.q{2} > 0/\
+      (*Fake.f1{2} = (Fake.n{2}, Fake.m{2}, Fake.q{2}, Fake.aa{2}, Fake.bb{2}, Fake.gg{2}) /\*)
+      borne = Fake.n{2} + Fake.q{2} /\
+      AdvAda.l{1} = borne-1 /\
+    (forall i, i >= Fake.n{2} => i < Fake.n{2}+Fake.q{2} => Fake.aa{2}.[i] >= 0 /\
+           Fake.bb{2}.[i] < borne /\ Fake.bb{2}.[i] < i /\ Fake.aa{2}.[i] < Fake.bb{2}.[i]) /\
+    (forall g, if (AdvAda.bb{1}.[g] = borne-1 /\ evalGate AdvAda.gg{1}.[g]
+      ((!AdvAda.v{1}.[AdvAda.aa{1}.[g]]), false) = evalGate AdvAda.gg{1}.[g] ((!AdvAda.v{1}.[AdvAda.aa{1}.[g]]), true)) then
+        AdvAda.yy{1}.[g]=proj Fake.randG{2}.[(g, true, false)] else true)/\
+
+    AdvAda.g{1} = Fake.g{2} /\
+      Fake.g{2} > Fake.n{2} /\
+    true
+  ).
+    admit.
+
+  wp.
+  while (
+      (glob ADV){1} = (glob ADV){2} /\
+      length AdvAda.xx{1} = AdvAda.n{1}+AdvAda.q{1} /\
+      length AdvAda.t{1} = AdvAda.n{1}+AdvAda.q{1} /\
+      AdvAda.xx{1} = Fake.xx{2} /\
+      AdvAda.t{1} = Fake.t{2}/\
+      AdvAda.v{1} = Fake.v{2}/\
+      AdvAda.n{1} = Fake.n{2}/\
+      AdvAda.m{1} = Fake.m{2}/\
+      AdvAda.q{1} = Fake.q{2}/\
+      AdvAda.aa{1} = Fake.aa{2}/\
+      AdvAda.bb{1} = Fake.bb{2}/\
+      AdvAda.randG{1} = Fake.randG{2}/\
+      AdvAda.pp{1} = Fake.pp{2}/\
+      AdvAda.fc{1} = Fake.f1{2}/\
+      (AdvAda.c{1} = DKC.Dkc.b{1}) = PrvInd.b{2}/\
+      AdvAda.xc{1} = Fake.x1{2}/\
+      Fake.n{2} > 1/\
+      Fake.m{2} > 0/\
+      Fake.q{2} > 0/\
+      (*Fake.f1{2} = (Fake.n{2}, Fake.m{2}, Fake.q{2}, Fake.aa{2}, Fake.bb{2}, Fake.gg{2}) /\*)
+      borne = Fake.n{2} + Fake.q{2} /\
+      AdvAda.l{1} = borne-1 /\
+    (forall i, i >= Fake.n{2} => i < Fake.n{2}+Fake.q{2} => Fake.aa{2}.[i] >= 0 /\
+           Fake.bb{2}.[i] < borne /\ Fake.bb{2}.[i] < i /\ Fake.aa{2}.[i] < Fake.bb{2}.[i]) /\
+
+    AdvAda.i{1} = Fake.i{2} /\
+      Fake.i{2} > 0 /\
+    true
+  );first (wp;skip;progress assumption;first (rewrite ! set_length;try assumption));smt.
+
+  while (
+      (glob ADV){1} = (glob ADV){2} /\
+      length AdvAda.xx{1} = AdvAda.n{1}+AdvAda.q{1} /\
+      length AdvAda.t{1} = AdvAda.n{1}+AdvAda.q{1} /\
+      AdvAda.xx{1} = Fake.xx{2} /\
+      AdvAda.t{1} = Fake.t{2}/\
+      AdvAda.v{1} = Fake.v{2}/\
+      AdvAda.n{1} = Fake.n{2}/\
+      AdvAda.m{1} = Fake.m{2}/\
+      AdvAda.q{1} = Fake.q{2}/\
+      AdvAda.aa{1} = Fake.aa{2}/\
+      AdvAda.bb{1} = Fake.bb{2}/\
+      AdvAda.randG{1} = Fake.randG{2}/\
+      AdvAda.pp{1} = Fake.pp{2}/\
+      AdvAda.fc{1} = Fake.f1{2}/\
+      (AdvAda.c{1} = DKC.Dkc.b{1}) = PrvInd.b{2}/\
+      AdvAda.xc{1} = Fake.x1{2}/\
+      Fake.n{2} > 1/\
+      Fake.m{2} > 0/\
+      Fake.q{2} > 0/\
+      (*Fake.f1{2} = (Fake.n{2}, Fake.m{2}, Fake.q{2}, Fake.aa{2}, Fake.bb{2}, Fake.gg{2}) /\*)
+      borne = Fake.n{2} + Fake.q{2} /\
+      AdvAda.l{1} = borne-1 /\
+    (forall i, i >= Fake.n{2} => i < Fake.n{2}+Fake.q{2} => Fake.aa{2}.[i] >= 0 /\
+           Fake.bb{2}.[i] < borne /\ Fake.bb{2}.[i] < i /\ Fake.aa{2}.[i] < Fake.bb{2}.[i]) /\
+
+    AdvAda.i{1} = Fake.i{2} /\
+      Fake.i{2} > 0 /\
+    true
+  );first (wp;rnd;wp;skip;progress assumption;first (rewrite ! set_length;try assumption));smt.
+
+  wp;rnd;rnd;rnd.
+  skip.
+  progress.
 
   (*INVALID*)
   rcondf {1} 18;first (intros _;wp;rnd;wp;rnd;rnd;skip;smt).
   rcondf {2} 1;[intros &m;skip;smt|].
   wp.
   kill{1} 1!17;first (wp;rnd 1%r cPtrue;wp;rnd 1%r cPtrue;rnd 1%r cPtrue;skip;progress;smt).
-  rnd.
-  skip;progress;smt.
+  rnd.*)
+  skip;progress assumption.
 save.
